record layer files (legacy crypto)

src/tls/Encode.fst
@@ -2,7 +2,12 @@ module Encode
 
 (* The "plain" file for CPA encryption (module ENC) *)
 (* provided by LHAE,
-   implementing LHAEPlain @| MAC @| padding when using MtE *)
+   implementing LHAEPlain @| MAC @| padding when using MtE
+   
+   When safeId, substituting zeros for plaintexts
+
+   16-01-04 verifies with temporary assumptions; TBC
+ *)
 
 open FStar.Seq
 open Platform
@@ -13,20 +18,23 @@ open TLSConstants
 open TLSInfo
 open Range
 
-type id = i:id { is_MtE i.aeAlg } 
+// for now, we EXCLUDE MACOnly
+
+type id = i:id { is_MtE i.aeAlg /\ pv_of_id i <> TLS_1p3 } 
 
 // tmp
-type tagt (i:id) = bytes 
+type tagt (i:id) = MAC.tag i
 
 (* Interface towards ENC (conditionally abstract) *)
 
 // the result of decrypting & decoding, with an abstract type for secrecy
+// should we index just by plaintext lengths, rather than ad & range?
 private type plain (i:id) (ad: LHAEPlain.adata i) (rg:range) = | Plain:
   f: LHAEPlain.plain i ad rg ->
   tag: tagt i ->
 
-  // did decoding succeeded? stateful? always true with RC4.
-  ok : bool { encAlg_of_id i = (Stream CoreCrypto.RC4_128, Fresh) ==> ok = true } -> 
+  // did decoding succeed? stateful? always true with RC4.
+  ok : bool { is_MACOnly i.aeAlg \/ (encAlg_of_id i = (Stream CoreCrypto.RC4_128, Fresh) ==> ok = true) } -> 
   plain i ad rg 
 
 val plainLength: i:id -> clen: nat { clen >= ivSize i } -> Tot nat
@@ -60,7 +68,7 @@ let macPlain_bytes i rg ad b =
 val macPlain: i:id -> r:frange i ->
   =ad:LHAEPlain.adata i ->
   =f:LHAEPlain.plain i ad r ->
-  Tot (tagt i) // ?(b:bytes{ safeId i })
+  Tot bytes // (tagt i) // ?(b:bytes{ safeId i })
 let macPlain i rg ad f =
   macPlain_bytes i rg ad (payload i rg ad f)
 
@@ -79,7 +87,8 @@ private ask !i,r,ad,b,p.
 
 //$ in F*, it may be better to maintain a separate log for each MAC instance.
 
-#if ideal
+(*
+//#if ideal
 type maconly_entry =
     i:id * ad:LHAEPlain.adata i * rg:range * tlen:nat *
      payload:bytes * text:bytes * p:LHAEPlain.plain i ad rg * MAC.tag
@@ -108,14 +117,16 @@ let rec maconly_mem i ad cl pl text tag (xs:list<maconly_entry>) =
         when i=i' && ad=ad' && cl=cl' && pl=pl' && text=text' && tag=tag' -> let x = (rg',p') in Some x
     | _::xs -> maconly_mem i ad cl pl text tag xs
     | [] -> None
-#endif
+//#endif
+*)
 
-val mac: i:id -> k:MAC.key (*i*) -> ad:LHAEPlain.adata i -> rg:range -> p:LHAEPlain.plain i ad rg ->  (plain i ad rg)
+val mac: i:id -> k:MAC.key i (fun _ -> True) -> ad:LHAEPlain.adata i -> rg:frange i -> p:LHAEPlain.plain i ad rg ->  (plain i ad rg)
 let mac i k ad rg plain =
     let p = LHAEPlain.makeExtPad i ad rg plain in
     let text = macPlain i rg ad p in
-    let tag  = MAC.mac i k text in
-#if ideal
+    let tag  = MAC.mac k text in
+(*
+//#if ideal
     (* For MACOnly ciphersuites where AuthId holds, we store the plain and
      * the tag in the MACOnly log *)
     let e_aealg = i.aeAlg in
@@ -128,81 +139,62 @@ let mac i k ad rg plain =
           maconly_log := (i,ad,rg,tlen,pl,text,p,tag)::!maconly_log
        | _ -> ())
      else ();
-#endif
-    {plain = p;
-     tag = tag;
-     ok = true
-    }
+//#endif
+*)
+    Plain p tag true
 
-(*MK 26/09/2015 restore at some point*)
 
-(*val verify_MACOnly:
-  e: id{ ~ (safeId e) /\ is_MACOnly e.aeAlg } ->
-  k: MAC.key ->
-  ad: LHAEPlain.adata e ->
-  rg: range ->
-  tlen: nat{
-    tlen <= max_TLSCipher_fragment_length /\//
-    rg = cipherRangeClass e tlen
-    } ->
-  b: rbytes rg ->
-  t: MAC.tag ->
-  result (LHAEPlain.plain e ad (cipherRangeClass e tlen))*)
+// val verify_MACOnly:
+//   e: id{ ~ (safeId e) /\ is_MACOnly e.aeAlg } ->
+//   k: MAC.key ->
+//   ad: LHAEPlain.adata e ->
+//   rg: range ->
+//   tlen: nat{
+//     tlen <= max_TLSCipher_fragment_length /\//
+//     rg = cipherRangeClass e tlen
+//     } ->
+//   b: rbytes rg ->
+//   t: MAC.tag ->
+//   result (LHAEPlain.plain e ad (cipherRangeClass e tlen))
+//
+// let verify_MACOnly (e:id) k (ad:LHAEPlain.adata e) (rg:range) (cl:nat) b tag 
+//   (*: result (LHAEPlain.plain e ad rg)*)
+//   =
+//   let text = macPlain_bytes e rg ad b in
+//   if MAC.verify e k text tag then
+//   #if ideal
+//     if authId e then
+//       match maconly_mem e ad cl b text tag !maconly_log with
+//       | Some(x) ->
+//           let (rg',p') = x in
+//           let p = LHAEPlain.widen e ad rg' p' in
+//           let rg = rangeClass e rg' in
+//           Correct p
+//       | None ->
+//           Error(AD_bad_record_mac,perror __SOURCE_FILE__ __LINE__ "")
+//     else
+//   #endif
+//           let p = LHAEPlain.mk_plain e ad rg b in
+//           Correct p
+//   else
+//           Error(AD_bad_record_mac,perror __SOURCE_FILE__ __LINE__ "")
 
-let verify_MACOnly (e:id) k (ad:LHAEPlain.adata e) (rg:range) (cl:nat) b tag 
-  (*: result (LHAEPlain.plain e ad rg)*)
+val verify:
+  i:id ->
+  k: MAC.key i (fun _ -> True) ->
+  ad: LHAEPlain.adata i ->
+  rg: frange i ->
+  p: plain i ad rg ->
+  Result (LHAEPlain.plain i ad rg)
 
-  =
-  let text = macPlain_bytes e rg ad b in
-  if MAC.verify e k text tag then
-  #if ideal
-    if authId e then
-      match maconly_mem e ad cl b text tag !maconly_log with
-      | Some(x) ->
-          let (rg',p') = x in
-          let p = LHAEPlain.widen e ad rg' p' in
-          let rg = rangeClass e rg' in
-          Correct p
-      | None ->
-          Error(AD_bad_record_mac,perror __SOURCE_FILE__ __LINE__ "")
-    else
-  #endif
-          let p = LHAEPlain.mk_plain e ad rg b in
-          Correct p
-  else
-          Error(AD_bad_record_mac,perror __SOURCE_FILE__ __LINE__ "")
-
-(*MK 26/09/2015 restore at some point*)
-
-(*val verify:
-  e:id ->
-  k: MAC.key ->
-  ad: LHAEPlain.adata e ->
-  rg: range ->
-  ps: plain e ad rg ->
-  result (LHAEPlain.plain e ad rg)*)
-let verify (e:id) k ad rg (plain:plain e ad rg) =
-    let f = plain.plain in
-    let text = macPlain e rg ad f in
-    let tag  = plain.tag in
+let verify (i:id) k ad rg p =
+    let text = macPlain i rg ad p.f in
         (*@ We implement standard mitigation for padding oracles.
             Still, we note a small timing leak here:
             The time to verify the mac is linear in the plaintext length. *)
-    if MAC.verify e k text tag && plain.ok then
-        match LHAEPlain.parseExtPad e ad rg f with
-        | Correct(f) -> correct f
-        | Error(x) ->
-            #if DEBUG
-            Error(AD_bad_record_mac,perror __SOURCE_FILE__ __LINE__ "")
-            #else
-            Error(AD_bad_record_mac,"")
-            #endif
-      else
-            #if DEBUG
-            Error(AD_bad_record_mac,perror __SOURCE_FILE__ __LINE__ "")
-            #else
-            Error(AD_bad_record_mac,"")
-            #endif
+    if MAC.verify k text p.tag && p.ok 
+    then Correct p.f 
+    else Error(AD_bad_record_mac,"")
 
 (* KB we need to add some refinement to ensure that verify
    will not fail for MACed values *)
@@ -223,138 +215,182 @@ let pad p  = createBytes p (Bytes.byte_of_int (p-1)) //TODO: NS REVIEW!
 // plain record ---encode---> plaintext bytes
 
 val encode:
-      e:id{ ~ (safeId e) } ->
-      tlen:nat {tlen <= max_TLSCipher_fragment_length} ->
-      rg:range {tlen = targetLength e rg} ->
-      ad: LHAEPlain.adata e ->
-      pl: LHAEPlain.plain e ad rg ->
-      tag: MAC.tag ->
-      Tot (lbytes (plainLength e tlen))
+      i:id{ ~ (authId i) } -> // was not safeId i
+      ad: LHAEPlain.adata i ->
+      rg:range {
+        snd rg <= max_TLSPlaintext_fragment_length /\ 
+        snd rg - fst rg <= maxPadSize i - minimalPadding i (snd rg + macSize (macAlg_of_id i)) } ->
+      pl: LHAEPlain.plain i ad rg ->
+      tag: MAC.tag i ->
+      Tot (lbytes (plainLength i (targetLength i rg)))
 
-let encode (e:id) (tlen:nat) (rg:range) (ad:LHAEPlain.adata e) pl tag =
-    let b = payload e rg ad pl in
-    match e.aeAlg with
+let encode i ad rg pl tag =
+    let tlen = targetLength i rg in
+    let b = payload i rg ad pl in
+    match i.aeAlg with
     // no padding
     | MACOnly(mac)
     | MtE (Stream CoreCrypto.RC4_128) mac ->
         let (_,h) = rg in
         assert(length b = h);
         let payload = b @| tag in
-        assert(length payload = tlen - ivSize e);
+        assert(length payload = tlen - ivSize i);
         payload
     // padding
     | MtE (Block alg) mac ->
-        let plen = tlen - length b - length tag - ivSize e in
-        assert(plen > 0 && plen <= 256);
+        let plen = tlen - length b - length tag - ivSize i in
+        // assert(0 < plen && plen <= 256);
         let payload = b @| tag @| pad plen in
-        assert(length payload = tlen - ivSize e);
+        // assert(length payload = tlen - ivSize i);
         payload
-
 // plain record <---decode--- plaintext bytes
 
+
 val decode:
-      e:id{ ~ (authId e) }  ->
-    	ad: LHAEPlain.adata e ->
-	    rg: range ->
-	    tlen: nat{
-        tlen - ivSize(e) >= ( macKeySize(macAlg_of_id e) + fixedPadSize e ) &&
-        rg = cipherRangeClass e tlen} ->
-	    payload: lbytes (plainLength e tlen) ->
-      p: plain e ad rg
-      { p.ok <==> payload = encode e tlen rg ad p.plain p.tag }
+      i:id{ ~ (authId i) }  -> 
+      ad: LHAEPlain.adata i ->
+      tlen: nat{ 
+        valid_clen i tlen /\ 
+        tlen - ivSize i >= macKeySize(macAlg_of_id i) + fixedPadSize i /\ 
+        ( let rg = cipherRangeClass i tlen in 
+//          StatefulPlain.wf_ad_rg i (LHAEPlain.parseAD ad) rg /\
+          snd rg - fst rg <= maxPadSize i - minimalPadding i (snd rg + macSize (macAlg_of_id i))) } ->
+      payload: lbytes (plainLength i tlen) ->
+      p: plain i ad (cipherRangeClass i tlen) 
+      { pv_of_id i <> SSL_3p0 ==> (p.ok <==> (payload = encode i ad (cipherRangeClass i tlen) p.f p.tag ))}
 
-let decode (e:id) (ad:LHAEPlain.adata e) (rg:range) (tlen:nat) payload =
-    match e.aeAlg with
-    // no padding
-    | MACOnly(hashAlg)
+
+assume val lemma_pad: lx: nat { lx < 256 } -> 
+  Lemma ((createBytes lx (Bytes.byte_of_int lx) @| createBytes 1 (Bytes.byte_of_int lx)) = pad (lx+1))
+  
+
+let decode i ad tlen payload =
+    let pv = pv_of_id i in 
+    let l = length payload in 
+    let lt = macSize (macAlg_of_id i) in 
+ 
+    let rg : frange i = cipherRangeClass i tlen in
+    assume(StatefulPlain.wf_ad_rg i (LHAEPlain.parseAD ad) rg);
+    match i.aeAlg with
+    // no padding: we expect l = lf + lt
+    | MACOnly hashAlg
     | MtE (Stream CoreCrypto.RC4_128) hashAlg ->
-        assert(tlen = length payload + ivSize e);
-        let (fragment, tag) = Bytes.split payload (length payload - macSize (macAlg_of_id e)) in
-        { plain = LHAEPlain.mk_plain e ad rg fragment;
-          tag   = tag;
-          ok    = true; }
+        assert(tlen = l + ivSize i);
+        let lf = l - lt in
+        let (fragment, tag) = Bytes.split payload lf in
+        lemma_split payload lf; // could be automated!
+        let p = LHAEPlain.mk_plain i ad rg fragment in
+        assume( ~ (safeId i)); // should follow from their definitions
+        assert(payload = encode i ad rg p tag); 
+        Plain p tag true
 
-    // padding
-    | MtE (Block(encAlg)) hashAlg ->
-        let fp = fixedPadSize e in
-        let pLen = length payload in
-        let (tmpdata, padlenb) = Bytes.split payload (pLen - fp) in
-        let padlen = int_of_bytes padlenb in
-        let padstart = pLen - (padlen + fp) in
-        let macstart = padstart - macSize (macAlg_of_id e) in
-        if macstart < 0 then
+    // padding: we expect l = lf + lt + lx + lp bytes and tlen = lf + lx
+    | MtE (Block encAlg) hashAlg -> 
+        let lp = fixedPadSize i in
+        assert(lp = 1);
+        let (ftx,b) = Bytes.split payload (l - lp) in
+        lemma_split payload (l - lp); // could be automated!
+        let lx = int_of_bytes b in
+        assert( lx >= 0 /\ lx < 256);
+        let lft = l - (lx + lp) in
+        let lf  = lft - lt in
+        if lf < 0 then
             (*@ Evidently padding has been corrupted, or has been incorrectly generated;
                 following TLS1.1 we fail later (see RFC5246 6.2.3.2 Implementation Note) *)
-            let (fragment, tag) = split tmpdata (pLen - macSize (macAlg_of_id e) - fp) in
-            { plain = LHAEPlain.mk_plain e ad rg fragment;
-              tag   = tag;
-              ok    = false; }
+            let (f, tag) = split ftx (l - lt - lp) in
+            lemma_split ftx (l - lt - lp);
+            let p = LHAEPlain.mk_plain i ad rg f in  
+            assume(payload <> encode i ad rg p tag );
+            Plain p tag false
         else
-            let (actual,pad) = split tmpdata padstart in
-            let correctPadding =
-              match pv_of_id e with
-              | TLS_1p0 | TLS_1p1 | TLS_1p2 ->
-                (*@ We note a small timing leak here: the run time of the following two
-                    lines depends on padding length. We could mitigate it by implementing
-                    constant time comparison up to maximum padding length.*)
-                  let expected = createBytes padlen (Bytes.byte_of_int padlen) in
-                  equalBytes expected pad
-
+            let (ft,x) = split ftx lft in
+            let correctPadding: c:bool { c /\ pv <> SSL_3p0 ==> (x @| b) = pad (lx+1) } =
+              match pv with
               | SSL_3p0 ->
                 (*@ Padding is random in SSL_3p0, no check to be done on its content.
                     However, its length should be at most one bs
                     (See sec 5.2.3.2 of SSL 3 draft). *)
-                  padlen + fp <= blockSize encAlg in
+                  lx + lp <= CoreCrypto.blockSize encAlg 
 
-            if correctPadding then
-                let (fragment, tag) = split actual macstart in
-                { plain = LHAEPlain.mk_plain e ad rg fragment;
-                  tag   = tag;
-                  ok    = true; }
-            else
-                let (fragment, tag) = split tmpdata (pLen - macSize (macAlg_of_id e) - fp) in
-                { plain = LHAEPlain.mk_plain e ad rg fragment;
-                  tag   = tag;
-                  ok    = false; }
+              | TLS_1p0 | TLS_1p1 | TLS_1p2 ->
+                (*@ We note a small timing leak here: the run time of the following two
+                    lines depends on padding length. We could mitigate it by implementing
+                    constant time comparison up to maximum padding length.*)
+                  let expected = createBytes lx (Bytes.byte_of_int lx) in
+                  if x = expected then
+                    ( lemma_pad lx; 
+                      assume(b = createBytes 1 (Bytes.byte_of_int lx));
+                      assert((x @| b) = pad (lx+1));
+                      true )
+                  else false 
 
+               | _ -> false in
+
+            if correctPadding then (
+                let (f, tag) = split ft lf in
+                lemma_split ft lf; 
+                assume(Within lf rg);
+                let p = LHAEPlain.mk_plain i ad rg f in  
+                assume (safeId i ==> authId i);
+                assume((pv <> SSL_3p0 /\
+                  (x @| b = pad (lx+1))) ==>
+                  (f @| tag @| (x @| b) = encode i ad rg p tag) /\
+                  payload = encode i ad rg p tag);
+                Plain p tag true )
+            else (
+                let lf = l - lt - lp in  // faking minimal padding (lx = 0)
+                assume(Within lf rg);
+                let (f, tag) = split ftx lf in
+                lemma_split ftx lf;
+                let p = LHAEPlain.mk_plain i ad rg f in
+                assume(payload <> encode i ad rg p tag );
+                Plain p tag false )
+
+(*
 // now almost as encode/decode... share?
 
 // minimal cipher length for MEE
-val minTlen: id -> Tot nat
-
-let minTlen i =
+let minTlen (i:id) =
   match i.aeAlg with
   | MACOnly hashAlg
   | MtE (Stream CoreCrypto.RC4_128) hashAlg -> macSize (macAlg_of_id i)
   | MtE (Block encAlg) hashAlg -> ivSize i + macSize (macAlg_of_id i) + fixedPadSize i
 
+(*
 // This property should follow by case analysis on all
 // enc/mac algorithms of TLS (see TLSConstants.fs7)
 let test1 _ = assert (forall e h. blockSize e <= macSize h)
 
 let test2 _ = assert (forall (i:id) enc mac.
     i.aeAlg = MtE (Block enc) mac ==> minTlen i >= blockSize enc)
+*)
 
 val mk_plain:
-  e:id{ ~ (authId e) } ->
-  ad: LHAEPlain.adata e ->
+  i:id{ ~ (authId i) } ->
+  ad: LHAEPlain.adata i ->
   tlen:nat{
-    tlen >= minTlen e &&
-    tlen <= max_TLSCipher_fragment_length } ->
-  lbytes (plainLength e tlen) ->
-  plain e ad (cipherRangeClass e tlen)
+    tlen >= minTlen i /\
+    tlen <= max_TLSCipher_fragment_length /\
+    valid_clen i tlen
+  } ->
+  lbytes (plainLength i tlen) ->
+  plain i ad (cipherRangeClass i tlen)
 
-let mk_plain (e:id) ad tlen b =
-  decode e ad (cipherRangeClass e tlen) tlen b
+let mk_plain i ad tlen b =
+  admit();
+  decode i ad tlen b
 
 val repr:
-  e:id{ ~ (safeId e) } ->
-  ad: LHAEPlain.adata e ->
-  rg:range -> //AP {rg is fRange}
-  plain e ad rg ->
-  b: lbytes (plainLength e (targetLength e rg))
-  { targetLength e rg <= max_TLSCipher_fragment_length }
+  i:id{ ~ (safeId i) } ->
+  ad: LHAEPlain.adata i ->
+  rg:range { snd rg <= max_TLSPlaintext_fragment_length /\ 
+             snd rg - fst rg <= maxPadSize i - minimalPadding i (snd rg + macSize (macAlg_of_id i)) } ->
+  plain i ad rg ->
+  b: lbytes (plainLength i (targetLength i rg))
+  { targetLength i rg <= max_TLSCipher_fragment_length }
   // should that be a property of targetLength?
 
-let repr (e:id) ad rg pl =
-  encode e (targetLength e rg) rg ad pl.plain pl.tag
+let repr i ad rg pl =
+  encode i ad rg pl.f pl.tag
+
+*)
